src/Util/Strings/Ascii.v
@@ -1,6 +1,10 @@
+Require Import Coq.NArith.NArith.
 Require Import Crypto.Util.Strings.Equality.
 Require Import Coq.Strings.Ascii.
+Require Import Crypto.Util.Notations.
 
+Local Open Scope bool_scope.
+Local Open Scope N_scope.
 Local Open Scope char_scope.
 
 (** Special characters *)
@@ -13,3 +17,18 @@ Example NewPage := "012".
 Example CR := "013".
 Example Escape := "027".
 Example NewLine := "010".
+
+Local Coercion N_of_ascii : ascii >-> N.
+Definition ltb (x y : ascii) : bool := N.ltb x y.
+Definition leb (x y : ascii) : bool := N.leb x y.
+Infix "<?" := ltb : char_scope.
+Infix "<=?" := leb : char_scope.
+
+Definition to_lower (ch : ascii) : ascii
+  := if ("A" <=? ch) && (ch <=? "Z")
+     then ascii_of_N ("a" + ch - "A")
+     else ch.
+Definition to_upper (ch : ascii) : ascii
+  := if ("a" <=? ch) && (ch <=? "z")
+     then ascii_of_N ("A" + ch - "a")
+     else ch.
